%        File: notes.tex
%     Created: Tue Jan 08 11:00 AM 2013 P
% Last Change: Tue Jan 08 11:00 AM 2013 P
%
\input{header.tex}
%\usepackage{hyperref}

\newcommand{\nnsum}[2]{\sum_{\langle #1 #2 \rangle}}
\newcommand{\cc}{\mathrm{c.c.}}
\newcommand{\nghbr}[2]{#1,\,#2}

\begin{document}

\section{Definitions}

\begin{equation}
  H = (1 - s) H_D + s H_P,
  \qquad
  0 \leq s \leq 1
  \label{def-h_qaa}
\end{equation}
\begin{equation}
  H_D = \sum_i \sigma^x_i
  \label{def-h_d}
\end{equation}
\begin{equation}
  H_P = \nnsum{i}{j} \sigma^z_i \sigma^z_j + \sum_i h_i \sigma^z_i,
  \qquad
  h_i \rightarrow h
  \label{def-h_p}
\end{equation}
\begin{equation}
  f_{ij} = \pd{}{h_j} \avg{\sigma^z_i}
  \sim \avg{\sigma^z_i \sigma^z_j}
  \label{def-f}
\end{equation}

\section{Perturbation theory for susceptibility}

Calculate $f_{ij}$ in first-order nondegenerate perturbation theory.
Let $\ket{\psi}$ be the ground state.
\begin{equation}
  \pd{}{h_j} \avg{\sigma_i}
  = \matrixel{\pd{\psi}{h_j}}{\sigma_i}{\psi} + \cc
  \label{}
\end{equation}
Let
$h_j \rightarrow h_j + \delta h_j$.
Then
$H_P \rightarrow H_P + \delta h_j \sigma_j$.
The first-order change in the ground state is
\begin{equation}
  \ket{\psi^{(1)}}
  = \delta h_j \sum_{n>0} \frac{\matrixel{n}{\sigma_j}{\psi}}{E_0 - E_n} \ket{n}.
  \label{}
\end{equation}
Therefore
\begin{align}
  \ket{\pd{\psi}{h_j}}
  &= \lim_{\delta h_j \rightarrow 0} \frac{1}{\delta h_j} \ket{\psi^{(1)}} \\
  &= \sum_{n>0} \frac{\matrixel{n}{\sigma_j}{\psi}}{E_0 - E_n} \ket{n}
  \label{}
\end{align}
and
\begin{equation}
  \pd{}{h_j} \avg{\sigma_i}
  = -2 \avg{\sigma_j \sum_{n>0} \frac{\ket{n} \bra{n}}{E_n - E_0} \sigma_i}
  \label{}
\end{equation}
where $\avg{\cdots}$ is the ground-state expectation value.

\begin{equation}
  H = \sum_n E_n \ket{n} \bra{n}
  \label{}
\end{equation}
Let
\begin{equation}
  \boxed{
  H^{\prime} \equiv H - E_0 \ket{\psi} \bra{\psi}
  }
  \label{}
\end{equation}
Then
\begin{equation}
  H^{\prime} - E_0 = \sum_{n>0} \left( E_n - E_0 \right) \ket{n} \bra{n}
  \label{}
\end{equation}
and
\begin{equation}
  \boxed{
  \pd{}{h_j} \avg{\sigma_i}
  = -2 \avg{\sigma_j \left( H^{\prime} - E_0 \right)^{-1} \sigma_i}
  }
  \label{}
\end{equation}

\section{Computational basis}

Let $\ket{n}$ be an eigenstate of
$\sigma_1 \otimes \sigma_2 \otimes \cdots \otimes \sigma_N$
such that
\begin{equation}
    \sum_{k=0}^N \left( \sigma_k + \frac{1}{2} \right) 2^k \ket{n} = n \ket{n}.
  \label{}
\end{equation}
i.e. $\ket{n}$ corresponds to the spin configuration obtained by taking 1
as spin up and 0 as spin down in the binary representation of $n$.
For example, with $N=3$,
\begin{align*}
  \ket{0} \equiv \ket{000}
  &\equiv
  \ket{\downarrow} \otimes
  \ket{\downarrow} \otimes
  \ket{\downarrow} \\
  \ket{1} \equiv \ket{001}
  &\equiv
  \ket{\downarrow} \otimes
  \ket{\downarrow} \otimes
  \ket{\uparrow} \\
  &\vdots \\
  \ket{7} \equiv \ket{111}
  &\equiv
  \ket{\uparrow} \otimes
  \ket{\uparrow} \otimes
  \ket{\uparrow}.
  \label{}
\end{align*}

\section{Energy minimization}

The ground-state energy $E_0$ is the minimum of the objective function
\begin{equation}
  f(\ket{\psi}) 
  \equiv \frac{\matrixel{\psi}{H}{\psi}}{\braket{\psi}{\psi}}
  \label{eq:energy}
\end{equation}
with respect to $\ket{\psi}$, i.e.
\begin{equation}
  E_0 = \min_{\ket{\psi}} f(\ket{\psi}).
  \label{}
\end{equation}
Let $\{\ket{n}\}$ be the computational basis and write
$\ket{\psi} = \sum_n c_n \ket{n}$.
Because $H$ is real and symmetric in this basis, the components $c_n$ may be
taken to be real, i.e. $c_n=c_n^*$.
Denote the diagonal elements of $H$ by $d_n \equiv H_{n n}$ and the off-diagonal
elements by $a_{n m} \equiv H_{n m}$.
The objective function becomes
\begin{equation}
  f(\ket{\psi})
  = \frac{\sum_n c_n^2 d_n + \sum_n c_n \sum_m a_{n m} c_m}{\sum_n c_n^2}.
  \label{}
\end{equation}
The gradient is given by
\begin{equation}
  \pd{f}{c_k}
  = \frac{2}{\braket{\psi}{\psi}}
  \left( \matrixel{k}{H}{\psi} - f c_k \right)
  \label{eq:grad}
\end{equation}
or
\begin{equation}
  \pd{f}{c_k}
  = \frac{2 c_k (d_k - f) + 2 \sum_m a_{k m} c_m}{\sum_n c_n^2}.
  \label{}
\end{equation}

\subsection{Applying the conjugate gradient method}

At each step of the algorithm we minimize the energy in the direction
$\ket{\delta}$, i.e. we compute
\begin{equation}
  \min_{\alpha} f( \ket{\psi} + \alpha \ket{\delta} )
  = \min_{\alpha}
  \frac{
      \matrixel{\psi}{H}{\psi}
      + 2 \alpha \matrixel{\delta}{H}{\psi}
      + \alpha^2 \matrixel{\delta}{H}{\delta}
    }
    {
      \braket{\psi}{\psi}
      + 2 \alpha \braket{\delta}{\psi}
      + \alpha^2 \braket{\delta}{\delta}
    }.
  \label{}
\end{equation}
The critical points are given by solutions of
\begin{equation}
  \left. \pd{}{\alpha} f(\ket{\psi} + \alpha \ket{\delta}) \right|_{\alpha=\alpha^*} = 0
  \label{}
\end{equation}
\begin{align}
  &{\alpha^*}^2 \left( \braket{\delta}{\psi} \matrixel{\delta}{H}{\delta}
    - \braket{\delta}{\delta} \matrixel{\psi}{H}{\delta} \right) \\
  &\alpha^* \left( \braket{\psi}{\psi} \matrixel{\delta}{H}{\delta}
    - \braket{\delta}{\delta} \matrixel{\psi}{H}{\psi} \right) \\
  &\phantom{\alpha^*(} \braket{\psi}{\psi} \matrixel{\delta}{H}{\psi}
    - \braket{\delta}{\psi} \matrixel{\psi}{H}{\psi} = 0
  \label{}
\end{align}

\section{Off-diagonal elements of $H$}
In the computational basis $H_P$ is diagonal, allowing computation of
$\avg{H_P}$ in $2^N$ steps. $H_D$ is non-diagonal but sparse; $\avg{H_D}$ may
be computed in $2^N \times N$ steps noting that $H_D$ connects states that
differ by a single spin flip:
\begin{equation}
  \matrixel{n}{H_D}{m}
  = \begin{cases}
    1 & \ket{n}, \ket{m} \text{ differ by a single spin flip} \\
    0
  \end{cases}
  \label{}
\end{equation}
For each state $\ket{n}$ there are $N$ ``neighboring'' states that differ by a
single spin flip. Let $\ket{\nghbr{n}{k}}$ denote the $k$th neighbor of
$\ket{n}$. We have
\begin{align}
  \matrixel{n}{H_D}{\psi}
  &= \sum_m \matrixel{n}{H_D}{m} \braket{m}{\psi} \\
  &= \sum_{k=1}^N \matrixel{n}{H_D}{\nghbr{n}{k}} \braket{\nghbr{n}{k}}{\psi} \\
  &= \sum_{k=1}^N \braket{\nghbr{n}{k}}{\psi}
  \label{eq:id}
\end{align}
and therefore
\begin{align}
  \avg{H_D}
  &= \sum_n \braket{\psi}{n} \matrixel{n}{H_D}{\psi} \\
  &= \sum_n \braket{\psi}{n} \sum_{k=1}^{N} \braket{\nghbr{n}{k}}{\psi}.
  \label{eq:avgHd}
\end{align}
Let $E_n$ denote the eigenvalue of $H_P$ corresponding to $\ket{n}$ and define
$\psi_{\nghbr{i}{k}} \equiv \braket{\nghbr{i}{k}}{\psi}$.
Then, combining \eqref{eq:energy} and \eqref{eq:avgHd}, we have
\begin{equation}
  \mathcal{E}
  = \frac{1}{\abs{\psi}^2}
  \left[
  (1-s) \sum_n \psi_n \sum_{k=1}^N \psi_{\nghbr{n}{k}}
  + s \sum_n \psi_n^2 E_n
  \right].
  \label{}
\end{equation}
Combining \eqref{eq:grad} and \eqref{eq:id}, we have 
\begin{equation}
  \pd{\mathcal{E}}{\psi_i}
  = \frac{2}{\abs{\psi}^2}
  \left[
      (1-s) \sum_{k=1}^N \psi_{\nghbr{i}{k}}
    - \left( 1 - \frac{E_i}{\mathcal{E}} s \right) \mathcal{E} \psi_i
  \right].
\end{equation}
\end{document}

